% Thanks to Dan Wang for the Beamer template!

\documentclass[9pt]{beamer}

% Fill in variables below %
% ++++++++++++++++++++++++++++++++++++++++++++++++++++++++++++++++++++++++++++ %
\newcommand{\thesemester}{Spring 2013}
\newcommand{\themidterm}{CS 70 Midterm 1 Review}
\newcommand{\theauthors}{Edwin Liao, Sung Roa Yoon}
\newcommand{\theorganization}{Eta Kappa Nu, Mu Chapter \\
University of California, Berkeley}
\newcommand{\thedate}{February 18, 2013}
\newcommand{\thelanguage}{Java}
% ++++++++++++++++++++++++++++++++++++++++++++++++++++++++++++++++++++++++++++ %

% Preamble %
% ---------------------------------------------------------------------------- %
\usepackage{url}
\usepackage{relsize}
\usepackage{color}
\usepackage{listings}
\usepackage{multirow}
\usepackage{array}
\usepackage{bm}
\usepackage{framed}
\usepackage{amsfonts}
\usepackage{amsmath}

% Listings Package %
\usepackage{listings}
\lstset{numbers=left,
    basicstyle=\ttfamily,
    numberstyle=\tiny,
    showstringspaces=false,
    frame=leftline,
    language=Java,
    escapeinside=\$\$,
    keywordstyle=\color{blue},
    xleftmargin=20pt,
    morecomment=[l]{//},
    }

\usetheme{Singapore}
\setbeamertemplate{mini frames}[circle]
\setbeamertemplate{footline}[frame number]


\title{\themidterm}
\author{\theauthors}
\institute{\theorganization}
\date{\thedate}
% ---------------------------------------------------------------------------- %

\begin{document}

% Title Page %
% ---------------------------------------------------------------------------- %

\begin{frame}[fragile]
  \titlepage
\end{frame}


% Propositions and Proof Techniques %
% ---------------------------------------------------------------------------- %
\section{Propositions and Proof Techniques}
\subsection{Propositions and Proof Techniques}

\begin{frame}[fragile]
  \frametitle{Proof by Awesomeness}
Given points (1, 0), (2, 1), (3, 0) over $GF(7)$, find the polynomial of degree 2 using Lagrange Interpolation. \newline
\uncover<2->{\alert<2>{
\begin{eqnarray}
\Delta_1 (x) &=& \text{\emph{Don't care!}} \nonumber \\
\Delta_2 (x) &=& \frac{(x-1)(x-3)}{(2-1)(2-3)} = -x^2 + 4x - 3 \nonumber \\
\Delta_3 (x) &=& \text{\emph{Don't care!}} \nonumber \\
p(x) &=& 0 \cdot \delta_1 + 1 \cdot \delta_2 + 0 \cdot \delta_3 = -x^2 + 4x -3 = 6x^2 + 4x + 4 \nonumber
\end{eqnarray}
}}
\end{frame}



% Induction %
% ---------------------------------------------------------------------------- %
\section{Induction}

\subsection{Summary}
\begin{frame}[fragile]
  \frametitle{Proofs by Induction}
  Prove by induction $\forall k \in \mathbb{N}, P(k)$, where $\sum\limits_{i=1}^k i = \frac{k(k+1)}{2}$ \\
  \uncover<2->{\alert<2>{
      Base Case: $P(1)$. Then $\sum\limits_{i=1}^1 i = \frac{1(1+1)}{2} = 1$ \\
  }}
  \uncover<3->{\alert<3>{
      Induction Hypothesis: Assume $P(m)$ for some $m$. \\
  }}
  \uncover<4->{\alert<4>{
      Induction Step: Prove for $P(m + 1)$. \\
      \begin{align}
      P(m + 1) &= P(m) + (m + 1)\nonumber \\
      &= \frac{m(m+1)}{2} + (m + 1) \nonumber \\
      &= \frac{m^2 + m + 2(m + 1)}{2} \nonumber \\
      &= \frac{m^2 + 3m + 2}{2}  \nonumber \\
      &= \frac{(m + 1) (m + 2)}{2}  \nonumber \\
      \end{align}
  }}
\end{frame}

\subsection{Question1}
\begin{frame}[fragile]
  \frametitle{Cubed $\rightarrow$ Squared}
  Prove by induction $\forall k \in \mathbb{N}, P(k)$, where $\sum\limits_{i=1}^k i^3 = (\frac{k(k+1)}{2})^2$ \\
  \uncover<2->{\alert<2->{
      Base Case: $P(1)$. Then $\sum\limits_{i=1}^1 i^3 = (\frac{1(1+1)}{2})^2 = 1$ \\
  }}
  \uncover<3->{\alert<3->{
      Induction Hypothesis: Assume $P(m)$ for some $m$. \\
  }}
  \uncover<4->{\alert<4>{
      Induction Step: Prove for $P(m + 1)$. \\
      \begin{align}
      P(m + 1) &= P(m) + (m + 1)^3\nonumber \\
      &= (\frac{m(m+1)}{2})^2 + (m + 1)^3 \nonumber \\
      &= \frac{m^2(m+1)^2}{4} + \frac{4(m+1)(m + 1)^2}{4} \nonumber \\
      &= \frac{(m^2 + 4m + 4)(m+1)^2}{4} \nonumber \\
      &= \frac{(m+2)^2(m+1)^2}{4} \nonumber \\
      &= (\frac{m+1)(m+2)}{2})^2 \nonumber
      \end{align}
  }}
\end{frame}

\subsection{Question2}
\begin{frame}[fragile]
  \frametitle{Chocolate}
  (Vazirani Fa12 Midterm 1 3b)
  You wish to break a standard $m × n$ Hershey chocolate bar into $mn$ little squares to distribute to $mn$ kids. In each step you can pick up exactly one piece of chocolate and break it along one
of the horizontal or vertical lines etched into the bar. No stacking! Prove by induction that the minimum number of steps required to completely break the bar into $mn$ little squares is
$mn - 1$.\newline \\
  \uncover<2->{\alert<2->{
      We will use induction on $r = mn$; induction on the number of pieces in the bar. \newline \\
  }}
  \uncover<3->{\alert<3->{
      Base Case: The minimum number of breaks required is $g(r)$. $r = 1$. $m = 1$, $n = 1$. No breaks are
necessary, and we observe that $g(r) = r - 1 = 0$. \newline \\
  }}
  \uncover<4->{\alert<4->{
      Induction Hypothesis: Assume $\forall s \leq k g(s) = s - 1$. (Strong induction)\newline \\
  }}
  \uncover<5->{\alert<5>{
      Induction Step: Prove for $P(m + 1)$. \\
      Consider $r = k + 1$. Since we have one big piece and $k + 1$ pieces to distribute, we need to begin by making 1 break. This results in two bars, one with $u < k + 1$ and another with
$v < k+1$ pieces, where $u+v = k+1$. Applying the inductive hypothesis, it takes a minimum of
$g(v) = v−1$ breaks on the bar of size $v$, and it takes $g(u) = u−1$ breaks on the bar of size $u$. The
total minimum number of breaks is then $g(k+1) = 1+(v−1)+(u−1) = (u+v)−1 = (k+1)−1$.
Therefore, for any bar of size $mn$, it takes a minimum of $mn − 1$ breaks. 
  }}
\end{frame}


% Stable Marriage %
% ---------------------------------------------------------------------------- %
\section{Stable Marriage}
\subsection{Stable Marriage}

\begin{frame}[fragile]
  \frametitle{Winning the Lottery}
\end{frame}


% Modular Arithmetic %
% ---------------------------------------------------------------------------- %
\section{Modular Arithmetic}
  \subsection{Modular Arithmetic}

\begin{frame}[fragile]
  \frametitle{\emph{En Taro} Tassadar}
\end{frame}


% Public Key Cryptography %
% ---------------------------------------------------------------------------- %
\section{Public Key Cryptography}
  \subsection{Public Key Cryptography}

\begin{frame}[fragile]
  \frametitle{\emph{En Taro} Tassadar}
\end{frame}

% The End %
% ---------------------------------------------------------------------------- %

\begin{frame}
  \frametitle{\huge{That's it!}}
\end{frame}

\end{document}
